removed segment length and limit resources

theories/iris/host/iris_host.v
@@ -515,10 +515,10 @@ Global Instance host_heapG_irisG `{ HHB:HandleBytes, !wasmG Σ, !hvisG Σ, !hmsG
       (ghost_map_auth haGName 1 (gmap_of_list fs)) ∗
       (ghost_map_auth frameGName 1 (<[ tt := f ]> ∅)) ∗ 
       (gen_heap_interp (gmap_of_list (fmap mem_length s.(s_mems)))) ∗
-      (gen_heap_interp (<[ () := seg_length s.(s_segs).(seg_data) ]> ∅)) ∗
+(*      (gen_heap_interp (<[ () := seg_length s.(s_segs).(seg_data) ]> ∅)) ∗ *)
       (gen_heap_interp (gmap_of_list (fmap tab_size s.(s_tables)))) ∗
       (@gen_heap_interp _ _ _ _ _ memlimit_hsG (gmap_of_list (fmap mem_max_opt s.(s_mems)))) ∗
-      (@gen_heap_interp _ _ _ _ _ seglimit_hsG (<[ () := seg_max_opt s.(s_segs) ]> ∅)) ∗
+(*      (@gen_heap_interp _ _ _ _ _ seglimit_hsG (<[ () := seg_max_opt s.(s_segs) ]> ∅)) ∗ *)
       (@gen_heap_interp _ _ _ _ _ tablimit_hsG (gmap_of_list (fmap table_max_opt s.(s_tables)))) ∗
       ⌜ wellFormedState s ⌝
     )%I;
@@ -927,7 +927,7 @@ Proof.
 
   iIntros (σ ns κ κs nt) "Hσ".
   destruct σ as [[[[ws vis] ms] ha] f].
-  iDestruct "Hσ" as "(Hf & Ht & Hm & Hs & Ha & Hg & Hvis & Hms & Hha & Hframe & Hmemlen & Hseglen & Htabsize & Hmemlim & Hseglim & Htablim)".
+  iDestruct "Hσ" as "(Hf & Ht & Hm & Hs & Ha & Hg & Hvis & Hms & Hha & Hframe & Hmemlen & Htabsize & Hmemlim & Htablim)".
   iDestruct (ghost_map_lookup with "Hms Hmod") as "%Hmodlookup".
   iSpecialize ("Hes1" with "Hmod").
   iSpecialize ("Hes1" $! (ws, vis, ms, ha, f) ns κ κs nt).
@@ -1058,18 +1058,18 @@ Proof.
   - by iApply ("IH" with "[$]").   
 Qed.
 
-Definition instantiation_resources_pre hs_mod m hs_imps v_imps t_imps wfs wts wms wss was wgs hs_exps : iProp Σ :=
+Definition instantiation_resources_pre hs_mod m hs_imps v_imps t_imps wfs wts wms wgs hs_exps : iProp Σ :=
   hs_mod ↪[mods] m ∗
   import_resources_host hs_imps v_imps ∗
-  instantiation_resources_pre_wasm m v_imps t_imps wfs wts wms wss was wgs ∗       
+  instantiation_resources_pre_wasm m v_imps t_imps wfs wts wms wgs ∗       
   export_ownership_host hs_exps ∗
   ⌜ length hs_exps = length m.(mod_exports) ⌝.
 
-Definition instantiation_resources_post hs_mod m hs_imps v_imps t_imps wfs wts wms wss was wgs hs_exps (idfstart: option nat) : iProp Σ :=
+Definition instantiation_resources_post hs_mod m hs_imps v_imps t_imps wfs wts wms wgs hs_exps (idfstart: option nat) : iProp Σ :=
   hs_mod ↪[mods] m ∗
   import_resources_host hs_imps v_imps ∗ (* vis, for the imports stored in host *)
   ∃ (inst: instance), 
-  instantiation_resources_post_wasm m v_imps t_imps wfs wts wms wss was wgs idfstart inst ∗       
+  instantiation_resources_post_wasm m v_imps t_imps wfs wts wms wgs idfstart inst ∗       
   module_export_resources_host hs_exps m.(mod_exports) inst. (* export resources, in the host store *)
 
 Lemma insert_exports_none_len vis iexps exps:
@@ -1133,26 +1133,26 @@ Qed.
 
 Section instantiation_spec.
   Context `{HHB : HandleBytes}.
-Lemma instantiation_spec_operational_no_start (s: stuckness) E (hs_mod: N) (hs_imps: list vimp) (v_imps: list module_export) (hs_exps: list vi) (m: module) t_imps t_exps wfs wts wms wss was wgs:
+Lemma instantiation_spec_operational_no_start (s: stuckness) E (hs_mod: N) (hs_imps: list vimp) (v_imps: list module_export) (hs_exps: list vi) (m: module) t_imps t_exps wfs wts wms wgs:
   m.(mod_start) = None ->
   module_typing m t_imps t_exps ->
   module_restrictions m ->
-  instantiation_resources_pre hs_mod m hs_imps v_imps t_imps wfs wts wms wss was wgs hs_exps -∗
+  instantiation_resources_pre hs_mod m hs_imps v_imps t_imps wfs wts wms wgs hs_exps -∗
   WP (([:: ID_instantiate hs_exps hs_mod hs_imps], [::]): host_expr) @ s; E
    {{ λ v: language.val wasm_host_lang, ⌜ v = immHV [] ⌝ ∗
-        instantiation_resources_post hs_mod m hs_imps v_imps t_imps wfs wts wms wss was wgs hs_exps None}}.
+        instantiation_resources_post hs_mod m hs_imps v_imps t_imps wfs wts wms wgs hs_exps None}}.
 Proof.
   
   move => Hmodstart Hmodtype Hmodrestr.
   assert (module_restrictions m) as Hmodrestr2 => //.
   
   iIntros "(Hmod & Himphost & Himpwasmpre & Hexphost & %Hlenexp)".
-  iDestruct "Himpwasmpre" as "(Himpwasm & Hseg & Hall & %Hebound & %Hdbound)".
+  iDestruct "Himpwasmpre" as "(Himpwasm & %Hebound & %Hdbound)".
   
   repeat rewrite weakestpre.wp_unfold /weakestpre.wp_pre /=.
   
   iIntros ([[[[ws vis] ms] has] f] ns κ κs nt) "Hσ".
-  iDestruct "Hσ" as "(Hwf & Hwt & Hwm & Hws & Hwa & Hwg & Hvis & Hms & Hhas & Hframe & Hmsize & Hssize & Htsize & Hmlimit & Hslimit & Htlimit & %HWF)".
+  iDestruct "Hσ" as "(Hwf & Hwt & Hwm & Hws & Hwa & Hwg & Hvis & Hms & Hhas & Hframe & Hmsize & Htsize & Hmlimit & Htlimit & %HWF)".
 
   (* module declaration *)
   iDestruct (ghost_map_lookup with "Hms Hmod") as "%Hmod".
@@ -1839,7 +1839,7 @@ Proof.
 
     (* Wasm state update, using the instantiation characterisation lemma *)
     iDestruct (instantiation_wasm_spec with "") as "H" => //.
-    iDestruct ("H" with "[Himpwasm Hall Hseg] [Hwf Hwt Hwm Hwg Hmsize Hssize Htsize Hmlimit Hslimit Htlimit]") as "Hq".
+    iDestruct ("H" with "[Himpwasm] [Hwf Hwt Hwm Hwg Hmsize Htsize Hmlimit Htlimit]") as "Hq".
     { unfold instantiation_resources_pre_wasm.
       by iFrame.
     }
@@ -1853,7 +1853,7 @@ Proof.
     iMod "Hq" as "(Hwasmpost & Hσ)".
     unfold gen_heap_wasm_store => /=.
     rewrite Halls Hsegs H0 => /=.
-    iDestruct "Hσ" as "(?&?&?&?&?&?&?&?&?&?)".
+    iDestruct "Hσ" as "(?&?&?&?&?&?&?&?)".
     iFrame.
 
     (* rewrite <- H3. *)
@@ -1894,25 +1894,25 @@ Proof.
 Qed.
 
 (* Instantiating modules with a start function. We combine the handling of sequence here all in one. *)
-Lemma instantiation_spec_operational_start_seq s E (hs_mod: N) (hs_imps: list vimp) (v_imps: list module_export) (hs_exps: list vi) (m: module) t_imps t_exps wfs wts wms wss was wgs nstart (Φ: language.val wasm_host_lang -> iProp Σ) idecls:
+Lemma instantiation_spec_operational_start_seq s E (hs_mod: N) (hs_imps: list vimp) (v_imps: list module_export) (hs_exps: list vi) (m: module) t_imps t_exps wfs wts wms wgs nstart (Φ: language.val wasm_host_lang -> iProp Σ) idecls:
   m.(mod_start) = Some (Build_module_start (Mk_funcidx nstart)) ->
   module_typing m t_imps t_exps ->
   module_restrictions m ->
   ↪[frame] empty_frame -∗                            
-  instantiation_resources_pre hs_mod m hs_imps v_imps t_imps wfs wts wms wss was wgs hs_exps -∗
-  (∀ idnstart, (↪[frame] empty_frame) -∗ (instantiation_resources_post hs_mod m hs_imps v_imps t_imps wfs wts wms wss was wgs hs_exps (Some idnstart)) -∗ WP ((idecls, [::AI_invoke idnstart]) : host_expr) @ s; E {{ Φ }}) -∗
+  instantiation_resources_pre hs_mod m hs_imps v_imps t_imps wfs wts wms wgs hs_exps -∗
+  (∀ idnstart, (↪[frame] empty_frame) -∗ (instantiation_resources_post hs_mod m hs_imps v_imps t_imps wfs wts wms wgs hs_exps (Some idnstart)) -∗ WP ((idecls, [::AI_invoke idnstart]) : host_expr) @ s; E {{ Φ }}) -∗
   WP (((ID_instantiate hs_exps hs_mod hs_imps) :: idecls, [::]): host_expr) @ s; E {{ Φ }}.
 Proof.
   move => Hmodstart Hmodtype Hmodrestr.
   assert (module_restrictions m) as Hmodrestr2 => //.
   
   iIntros "Hframeown (Hmod & Himphost & Himpwasmpre & Hexphost & %Hlenexp) Hwpstart".
-  iDestruct "Himpwasmpre" as "(Himpwasm & Hseg & Hall & %Hebound & %Hdbound)".
+  iDestruct "Himpwasmpre" as "(Himpwasm & %Hebound & %Hdbound)".
   
   repeat rewrite weakestpre.wp_unfold /weakestpre.wp_pre /=.
   
   iIntros ([[[[ws vis] ms] has] f] ns κ κs nt) "Hσ".
-  iDestruct "Hσ" as "(Hwf & Hwt & Hwm & Hws & Hwa & Hwg & Hvis & Hms & Hhas & Hframe & Hmsize & Hssize & Htsize & Hmlimit & Hslimit & Htlimit & %HWF)".
+  iDestruct "Hσ" as "(Hwf & Hwt & Hwm & Hws & Hwa & Hwg & Hvis & Hms & Hhas & Hframe & Hmsize & Htsize & Hmlimit & Htlimit & %HWF)".
 
   (* module declaration *)
   iDestruct (ghost_map_lookup with "Hms Hmod") as "%Hmod".
@@ -2673,7 +2673,7 @@ Proof.
 
     (* Wasm state update, using the instantiation characterisation lemma *)
     iDestruct (instantiation_wasm_spec with "") as "H" => //.
-    iDestruct ("H" with "[Himpwasm Hseg Hall] [Hwf Hwt Hwm Hwg Hmsize Hssize Htsize Hmlimit Hslimit Htlimit]") as "Hq".
+    iDestruct ("H" with "[Himpwasm] [Hwf Hwt Hwm Hwg Hmsize Htsize Hmlimit Htlimit]") as "Hq".
     { unfold instantiation_resources_pre_wasm.
       by iFrame.
     }
@@ -2686,7 +2686,7 @@ Proof.
     iMod "Hq" as "(Hwasmpost & Hσ)".
     unfold gen_heap_wasm_store => /=.
     rewrite Halls Hsegs H0 => /=.
-    iDestruct "Hσ" as "(?&?&?&?&?&?&?&?&?&?)".
+    iDestruct "Hσ" as "(?&?&?&?&?&?&?&?)".
     iFrame.
 
     (* rewrite <- H3. *)
@@ -2725,13 +2725,13 @@ Proof.
     by iFrame.
 Qed.
     
-Lemma instantiation_spec_operational_start s E (hs_mod: N) (hs_imps: list vimp) (v_imps: list module_export) (hs_exps: list vi) (m: module) t_imps t_exps wfs wts wms wss was wgs nstart (Φ: language.val wasm_host_lang -> iProp Σ):
+Lemma instantiation_spec_operational_start s E (hs_mod: N) (hs_imps: list vimp) (v_imps: list module_export) (hs_exps: list vi) (m: module) t_imps t_exps wfs wts wms wgs nstart (Φ: language.val wasm_host_lang -> iProp Σ):
   m.(mod_start) = Some (Build_module_start (Mk_funcidx nstart)) ->
   module_typing m t_imps t_exps ->
   module_restrictions m ->
   ↪[frame] empty_frame -∗                            
-  instantiation_resources_pre hs_mod m hs_imps v_imps t_imps wfs wts wms wss was wgs hs_exps -∗
-  (∀ idnstart, (↪[frame] empty_frame) -∗ (instantiation_resources_post hs_mod m hs_imps v_imps t_imps wfs wts wms wss was wgs hs_exps (Some idnstart)) -∗ WP (([::], [::AI_invoke idnstart]) : host_expr) @ s; E {{ Φ }}) -∗
+  instantiation_resources_pre hs_mod m hs_imps v_imps t_imps wfs wts wms wgs hs_exps -∗
+  (∀ idnstart, (↪[frame] empty_frame) -∗ (instantiation_resources_post hs_mod m hs_imps v_imps t_imps wfs wts wms wgs hs_exps (Some idnstart)) -∗ WP (([::], [::AI_invoke idnstart]) : host_expr) @ s; E {{ Φ }}) -∗
   WP (([:: ID_instantiate hs_exps hs_mod hs_imps], [::]): host_expr) @ s; E {{ Φ }}.
 Proof.
   iIntros.
