theories/iris/language/iris_wp_def.v
@@ -47,9 +47,9 @@ Class wasmG Σ :=
 
       seg_gen_hsG :> ghost_mapG Σ N (byte * btag);
 
-      segsize_gen_hsG :> gen_heapGS unit N Σ;
+(*      segsize_gen_hsG :> gen_heapGS unit N Σ;
 
-      seglimit_hsG :> gen_heapGS unit (option N) Σ;
+      seglimit_hsG :> gen_heapGS unit (option N) Σ; *)
 
       (*      alloc_gen_hsG :> gen_heapGS N (N*N) Σ; *)
       allGName : gname;
@@ -90,10 +90,10 @@ Definition gen_heap_wasm_store `{!wasmG Σ} (s: store_record) : iProp Σ :=
 (*   (ghost_map_auth allGName 1 (gmap_of_allocator s.(s_alls))) ∗ *)
    (gen_heap_interp (gmap_of_list s.(s_globals))) ∗
    (gen_heap_interp (gmap_of_list (fmap mem_length s.(s_mems)))) ∗
-   (gen_heap_interp ({[ () := seg_length s.(s_segs).(seg_data)]} : gmap unit N)) ∗
+(*   (gen_heap_interp ({[ () := seg_length s.(s_segs).(seg_data)]} : gmap unit N)) ∗ *)
    (gen_heap_interp (gmap_of_list (fmap tab_size s.(s_tables)))) ∗
    (@gen_heap_interp _ _ _ _ _ memlimit_hsG (gmap_of_list (fmap mem_max_opt s.(s_mems)))) ∗
-   (@gen_heap_interp _ _ _ _ _ seglimit_hsG ({[ () := seg_max_opt s.(s_segs)]} : gmap unit (option N))) ∗
+(*   (@gen_heap_interp _ _ _ _ _ seglimit_hsG ({[ () := seg_max_opt s.(s_segs)]} : gmap unit (option N))) ∗ *)
    (@gen_heap_interp _ _ _ _ _ tablimit_hsG (gmap_of_list (fmap table_max_opt s.(s_tables)))))%I.
 
 Global Instance heapG_irisG `{!wasmG Σ} : irisGS wasm_lang Σ := {
@@ -110,10 +110,10 @@ Global Instance heapG_irisG `{!wasmG Σ} : irisGS wasm_lang Σ := {
       (gen_heap_interp (gmap_of_list s.(s_globals))) ∗
       (ghost_map_auth frameGName 1 (<[ tt := Build_frame locs inst ]> ∅)) ∗ 
       (gen_heap_interp (gmap_of_list (fmap mem_length s.(s_mems)))) ∗
-      (gen_heap_interp ({[ () := seg_length s.(s_segs).(seg_data) ]} : gmap unit N)) ∗
+(*      (gen_heap_interp ({[ () := seg_length s.(s_segs).(seg_data) ]} : gmap unit N)) ∗ *)
       (gen_heap_interp (gmap_of_list (fmap tab_size s.(s_tables)))) ∗
       (@gen_heap_interp _ _ _ _ _ memlimit_hsG (gmap_of_list (fmap mem_max_opt s.(s_mems)))) ∗
-      (@gen_heap_interp _ _ _ _ _ seglimit_hsG ({[ () := seg_max_opt s.(s_segs) ]} : gmap unit (option N))) ∗
+(*      (@gen_heap_interp _ _ _ _ _ seglimit_hsG ({[ () := seg_max_opt s.(s_segs) ]} : gmap unit (option N))) ∗ *)
       (@gen_heap_interp _ _ _ _ _ tablimit_hsG (gmap_of_list (fmap table_max_opt s.(s_tables)))) ∗
       ⌜ wellFormedState s ⌝
      )%I;
@@ -157,10 +157,10 @@ Notation " ↦[ws]{ q }[ i ] v" := (ghost_map_elem segGName i q v)
                                    (at level 20, q at level 5, format " ↦[ws]{ q }[ i ] v") : bi_scope.
 Notation " ↦[ws][ i ] v" := (ghost_map_elem segGName i (DfracOwn 1) v)
                               (at level 20, format " ↦[ws][ i ] v"): bi_scope.
-Notation " ↦[wslength] v" := (mapsto (L:=unit) (V:=N) () (DfracOwn 1) v%V)
+(*Notation " ↦[wslength] v" := (mapsto (L:=unit) (V:=N) () (DfracOwn 1) v%V)
                                (at level 20, format " ↦[wslength] v"): bi_scope.
-Notation " ↪[wslimit] v" := (mapsto (L:=unit) (V:=option N) (hG:=seglimit_hsG) () (DfracDiscarded) v % V)
-                              (at level 20, format " ↪[wslimit] v") : bi_scope.
+Notation " ↪[wslimit] v" := (mapsto (L:=unit) (V:=option N) (hG:=seglimit_hsG) () (DfracDiscarded) v % V)  
+                              (at level 20, format " ↪[wslimit] v") : bi_scope. *)
 (* Notation "n ↣[allocated]{ q } v" := (mapsto (L:=N) (V:=N*N) n q v%V)
                                       (at level 20, q at level 5, format "n ↣[allocated]{ q } v") : bi_scope.
 Notation "n ↣[allocated] v" := (mapsto (L:=N) (V:=N*N) n (DfracOwn 1) v%V)
@@ -191,8 +191,8 @@ Definition mem_block_at_pos `{!wasmG Σ} (n: N) (l:bytes) k :=
   ([∗ list] i ↦ b ∈ l, n ↦[wm][ (N.of_nat (N.to_nat k+i)) ] b)%I.
 
 Definition seg_block `{!wasmG Σ} (s: segment) :=
-  (([∗ list] i ↦ b ∈ (s.(seg_data).(segl_data)), ↦[ws][ (N.of_nat i) ] b ) ∗
-      ↦[wslength] seg_length s.(seg_data) ∗  ↪[wslimit] (seg_max_opt s))%I.
+  (([∗ list] i ↦ b ∈ (s.(seg_data).(segl_data)), ↦[ws][ (N.of_nat i) ] b ) (* ∗
+       ↦[wslength] seg_length s.(seg_data) ∗  ↪[wslimit] (seg_max_opt s) *))%I.
 
 Definition seg_block_at_pos `{!wasmG Σ} (l:list (byte * btag)) k :=
   ([∗ list] i ↦ b ∈ l, ↦[ws][ (N.of_nat (N.to_nat k+i)) ] b)%I.
@@ -231,7 +231,7 @@ Proof.
 Qed.
 
 Definition seg_equiv (s1 s2: segment) : Prop :=
-  s1.(seg_max_opt) = s2.(seg_max_opt) /\
+  (* s1.(seg_max_opt) = s2.(seg_max_opt) /\ *)
     s1.(seg_data).(segl_data) = s2.(seg_data).(segl_data).
 
 Lemma seg_equiv_wsblock_rewrite `{!wasmG Σ} (s1 s2: segment):
@@ -241,7 +241,7 @@ Proof.
   unfold seg_equiv, seg_block.
   destruct s1, s2.
   destruct seg_data, seg_data0 => //=.
-  by move => [-> ->] => //.
+  by intros ->. (* by move => [-> ->] => //. *)
 Qed.
 
 
